---
title: "Deriving bias"
format: pdf
editor: visual
---

Deriving the bias of between and within effect in a twin fixed effects model:

twin j clustered in family i
$$
\begin{align}
Y_{ij}=b_{yx}X_{ij}+a_{21}A^{x}_{ij}+c_{21}C^{x}_{ij}+a_{22}A^{y}_{ij}+c_{22}C^{y}_{ij}+e_{22}E^{y}_{ij} \\
X_{ij}=a_{11}A^{x}_{ij}+c_{11}C^{x}_{ij}+e_{11}E^{x}_{ij} \\
Cov(C^{x}_{ij},C^{x}_{ij'})=1\\
Cov(A^{x}_{ij},A^{x}_{ij'})=r\\
Cov(C^{y}_{ij},C^{y}_{ij'})=1\\
Cov(A^{y}_{ij},A^{y}_{ij'})=r_{g}
\end{align}
$$

$$
\begin{align}
\beta_{w}=\frac{Cov(Y_{ij}, (X_{ij}-\bar{X}_{i}))}{Var(X_{ij}-\bar{X}_{i})} \\ 
=\frac{Cov\left[ Y_{ij},\left(\frac{X_{ij}-X_{ij'}}{2}\right)\right]}{Var\left(\frac{X_{ij}-X_{ij'}}{2}\right)} \\
=\frac{\frac{1}{2}[Cov(Y_{ij},X_{ij})-Cov(Y_{ij},X_{ij'})]}{\frac{1}{4}[2Var(X_{ij})-2Cov(X_{ij}, X_{ij'})]}\\
=\frac{Cov(b_{yx}X_{ij}+a_{21}A^{x}_{ij}+c_{21}C^{x}_{ij}+a_{22}A^{y}_{ij}+c_{22}C^{y}_{ij}+e_{22}E^{y}_{ij},X_{ij})-Cov(b_{yx}X_{ij}+a_{21}A^{x}_{ij}+c_{21}C^{x}_{ij}+a_{22}A^{y}_{ij}+c_{22}C^{y}_{ij}+e_{22}E^{y}_{ij},X_{ij'})}{Var(X_{ij})-Cov(X_{ij}, X_{ij'})}\\
=\frac{Cov(b_{yx}X_{ij}+a_{21}A^{x}_{ij}+c_{21}C^{x}_{ij}+a_{22}A^{y}_{ij}+c_{22}C^{y}_{ij}+e_{22}E^{y}_{ij},X_{ij})-Cov(b_{yx}X_{ij}+a_{21}A^{x}_{ij}+c_{21}C^{x}_{ij}+a_{22}A^{y}_{ij}+c_{22}C^{y}_{ij}+e_{22}E^{y}_{ij},X_{ij'})}{Var(X_{ij})-Cov(X_{ij}, X_{ij'})}\\
=\frac{b_{yx}(Var(X_{ij})-Cov(X_{ij},X_{ij'}))+a_{21}(Cov(A^{x}_{ij},X_{ij})-Cov(A^{x}_{ij},X_{ij'}))+c_{21}(Cov(C^{x}_{ij},X_{ij})-Cov(C^{x}_{ij},X_{ij'}))}{Var(X_{ij})-Cov(X_{ij}, X_{ij'})}\\
=b_{yx}+\frac{a_{21}(Cov(A^{x}_{ij},X_{ij})-Cov(A^{x}_{ij},X_{ij'}))+c_{21}(Cov(C^{x}_{ij},X_{ij})-Cov(C^{x}_{ij},X_{ij'}))}{Var(X_{ij})-Cov(X_{ij}, X_{ij'})}\\
=b_{yx}+\frac{a_{21}(a_{11}-r_{g}a_{11})}{a_{11}^{2}+c_{11}^{2}+e_{11}^{2}-(r_{g}a_{11}^{2}+c_{11}^{2})}
\end{align}
$$
For MZ twins, with $r_{g}=1$:
$$
\begin{align}
\beta_{w}^{MZ}=b_{yx}+\frac{a_{21}(a_{11}-a_{11})}{a_{11}^{2}+c_{11}^{2}+e_{11}^{2}-(a_{11}^{2}+c_{11}^{2})}
=b_{yx}
\end{align}
$$


For DZ twins, with $r_{g}=0.5$:
$$
\begin{align}
\beta_{w}^{DZ}=b_{yx}+\frac{a_{21}(a_{11}-0.5a_{11})}{a_{11}^{2}+c_{11}^{2}+e_{11}^{2}-(0.5a_{11}^{2}+c_{11}^{2})}\\
=b_{yx}+\frac{a_{21}0.5a_{11}}{0.5a_{11}^{2}+e_{11}^{2}}
\end{align}
$$
